src/MessageViewWf.v
@@ -1,0 +1,105 @@
+From hahn Require Import Hahn.
+Require Import PromisingLib.
+From Promising2 Require Import Memory View Time Cell TView.
+Require Import MemoryAux.
+
+Definition message_view_wf memory :=
+  forall loc to from val released
+         (GET : Memory.get loc to memory = 
+                Some (from, Message.full val released)),
+    View.opt_wf released.
+
+Lemma message_view_wf_add
+      memory loc from to msg memory'
+      (REL_WF : message_view_wf memory)
+      (PROM : Memory.add memory loc from to msg memory') :
+  message_view_wf memory'.
+Proof.
+  red. ins.
+  erewrite Memory.add_o in GET; eauto.
+  desf.
+  2: by eapply REL_WF; eauto.
+  simpls; desf.
+  inv PROM. inv ADD. inv MSG_WF.
+Qed.
+
+Lemma message_view_wf_split
+      memory loc from to to' msg msg' memory'
+      (REL_WF : message_view_wf memory)
+      (PROM : Memory.split memory loc from to to' msg msg' memory') :
+  message_view_wf memory'.
+Proof.
+  red. ins.
+  erewrite Memory.split_o in GET; eauto.
+  desf.
+  3: by eapply REL_WF; eauto.
+  all: simpls; desf.
+  { inv PROM. inv SPLIT. inv MSG_WF. }
+  inv PROM. inv SPLIT.
+  eapply REL_WF.
+  apply GET2.
+Qed.
+
+Lemma message_view_wf_lower
+      memory loc from to msg msg' memory'
+      (REL_WF : message_view_wf memory)
+      (PROM : Memory.lower memory loc from to msg msg' memory') :
+  message_view_wf memory'.
+Proof.
+  red. ins.
+  erewrite Memory.lower_o in GET; eauto.
+  desf.
+  2: by eapply REL_WF; eauto.
+  simpls; desf.
+  inv PROM. inv LOWER. inv MSG_WF.
+Qed.
+
+Lemma message_view_wf_op
+      memory loc from to msg memory' kind
+      (REL_WF : message_view_wf memory)
+      (PROM : Memory.op memory loc from to msg memory' kind) :
+  message_view_wf memory'.
+Proof.
+  destruct PROM.
+  { eapply message_view_wf_add; eauto. }
+  { eapply message_view_wf_split; eauto. }
+  eapply message_view_wf_lower; eauto.
+Qed.
+
+Lemma message_view_wf_promise
+      promises memory loc from to msg promises' memory' kind
+      (REL_WF : message_view_wf memory)
+      (PROM : Memory.promise promises memory loc from to
+                             msg promises' memory' kind) :
+  message_view_wf memory'.
+Proof.
+  destruct PROM.
+  { eapply message_view_wf_add; eauto. }
+  { eapply message_view_wf_split; eauto. }
+  eapply message_view_wf_lower; eauto.
+Qed.
+
+Lemma message_view_wf_init : message_view_wf Memory.init.
+Proof.
+  red. ins. apply memory_init_o in GET. desf.
+  unfold Message.elt in *. desf.
+Qed.
+
+Lemma message_view_wf_future memory memory'
+      (MVW    : message_view_wf memory)
+      (FUTURE : Memory.future memory memory') :
+  message_view_wf memory'.
+Proof.
+  induction FUTURE; auto.
+  apply IHFUTURE.
+  destruct H.
+  eapply message_view_wf_op; eauto.
+Qed.
+
+Lemma message_view_wf_future_init memory
+      (FUTURE : Memory.future Memory.init memory) :
+  message_view_wf memory.
+Proof.
+  eapply message_view_wf_future; eauto.
+  apply message_view_wf_init.
+Qed.
