src/SimulationRel.v
@@ -11,7 +11,7 @@ From imm Require Import CombRelations.
 From imm Require Import TraversalConfig.
 From imm Require Import MaxValue.
 From imm Require Import ViewRel.
-From imm Require Import Event_imm_promise.
+Require Import Event_imm_promise.
 From imm Require Import PromiseLTS.
 From imm Require Import ProgToExecution.
 From imm Require Import ProgToExecutionProperties.
